theories/heap_lang/lifting.v
@@ -3,11 +3,13 @@ From iris.proofmode Require Import tactics.
 From iris.algebra Require Import auth gmap.
 From iris.base_logic Require Export gen_heap.
 From iris.base_logic.lib Require Export proph_map.
-From iris.program_logic Require Export weakestpre.
-From iris.program_logic Require Import ectx_lifting total_ectx_lifting.
-From iris.heap_lang Require Export lang.
-From iris.heap_lang Require Import tactics notation.
+From diris.program_logic Require Export weakestpre.
+From diris.program_logic Require Import ectx_lifting.
+From diris.heap_lang Require Export lang.
 Set Default Proof Using "Type".
+From diris.heap_lang Require Import notation.
+From diris.heap_lang Require Import tactics.
+
 
 Class heapG Σ := HeapG {
   heapG_invG : invG Σ;
@@ -103,27 +105,6 @@ Instance cmpxchg_atomic s v0 v1 v2 : Atomic s (CmpXchg (Val v0) (Val v1) (Val v2
 Proof. solve_atomic. Qed.
 Instance faa_atomic s v1 v2 : Atomic s (FAA (Val v1) (Val v2)).
 Proof. solve_atomic. Qed.
-
-Instance new_proph_atomic s : Atomic s NewProph.
-Proof. solve_atomic. Qed.
-Instance resolve_atomic s e v1 v2 :
-  Atomic s e → Atomic s (Resolve e (Val v1) (Val v2)).
-Proof.
-  rename e into e1. intros H σ1 e2 κ σ2 efs [Ks e1' e2' Hfill -> step].
-  simpl in *. induction Ks as [|K Ks _] using rev_ind; simpl in Hfill.
-  - subst. inversion_clear step. by apply (H σ1 (Val v) κs σ2 efs), head_prim_step.
-  - rewrite fill_app. rewrite fill_app in Hfill.
-    assert (∀ v, Val v = fill Ks e1' → False) as fill_absurd.
-    { intros v Hv. assert (to_val (fill Ks e1') = Some v) as Htv by by rewrite -Hv.
-      apply to_val_fill_some in Htv. destruct Htv as [-> ->]. inversion step. }
-    destruct K; (inversion Hfill; clear Hfill; subst; try
-      match goal with | H : Val ?v = fill Ks e1' |- _ => by apply fill_absurd in H end).
-    refine (_ (H σ1 (fill (Ks ++ [K]) e2') _ σ2 efs _)).
-    + destruct s; intro Hs; simpl in *.
-      * destruct Hs as [v Hs]. apply to_val_fill_some in Hs. by destruct Hs, Ks.
-      * apply irreducible_resolve. by rewrite fill_app in Hs.
-    + econstructor 1 with (K := Ks ++ [K]); try done. simpl. by rewrite fill_app.
-Qed.
 
 Local Ltac solve_exec_safe := intros; subst; do 3 eexists; econstructor; eauto.
 Local Ltac solve_exec_puredet := simpl; intros; by inv_head_step.
@@ -221,19 +202,11 @@ Implicit Types l : loc.
 
 (** Fork: Not using Texan triples to avoid some unnecessary [True] *)
 Lemma wp_fork s E e Φ :
-  ▷ WP e @ s; ⊤ {{ _, True }} -∗ ▷ Φ (LitV LitUnit) -∗ WP Fork e @ s; E {{ Φ }}.
+  ▷ WP e @ s; ⊤ {{ _, True }} -∗ ▷ Φ (LitV LitUnit) -∗ WP Fork e @ s; E {{ Φ }}.  
 Proof.
-  iIntros "He HΦ". iApply wp_lift_atomic_head_step; [done|].
+  iIntros "He HΦ /=". iApply wp_lift_atomic_head_step; [done|].
   iIntros (σ1 κ κs n) "Hσ !>"; iSplit; first by eauto.
   iNext; iIntros (v2 σ2 efs Hstep); inv_head_step. by iFrame.
-Qed.
-
-Lemma twp_fork s E e Φ :
-  WP e @ s; ⊤ [{ _, True }] -∗ Φ (LitV LitUnit) -∗ WP Fork e @ s; E [{ Φ }].
-Proof.
-  iIntros "He HΦ". iApply twp_lift_atomic_head_step; [done|].
-  iIntros (σ1 κs n) "Hσ !>"; iSplit; first by eauto.
-  iIntros (κ v2 σ2 efs Hstep); inv_head_step. by iFrame.
 Qed.
 
 (** Heap *)
@@ -243,7 +216,7 @@ Lemma heap_array_to_seq_meta l vs (n : nat) :
   length vs = n →
   ([∗ map] l' ↦ _ ∈ heap_array l vs, meta_token l' ⊤) -∗
   [∗ list] i ∈ seq 0 n, meta_token (l +ₗ (i : nat)) ⊤.
-Proof.
+Proof. 
   iIntros (<-) "Hvs". iInduction vs as [|v vs] "IH" forall (l)=> //=.
   rewrite big_opM_union; last first.
   { apply map_disjoint_spec=> l' v1 v2 /lookup_singleton_Some [-> _].
@@ -289,36 +262,12 @@ Proof.
   - by iApply heap_array_to_seq_mapsto.
   - iApply (heap_array_to_seq_meta with "Hm"). by rewrite replicate_length.
 Qed.
-Lemma twp_allocN_seq s E v n :
-  0 < n →
-  [[{ True }]] AllocN (Val $ LitV $ LitInt $ n) (Val v) @ s; E
-  [[{ l, RET LitV (LitLoc l); [∗ list] i ∈ seq 0 (Z.to_nat n),
-      (l +ₗ (i : nat)) ↦ v ∗ meta_token (l +ₗ (i : nat)) ⊤ }]].
-Proof.
-  iIntros (Hn Φ) "_ HΦ". iApply twp_lift_atomic_head_step_no_fork; auto.
-  iIntros (σ1 κs k) "[Hσ Hκs] !>"; iSplit; first by destruct n; auto with lia.
-  iIntros (κ v2 σ2 efs Hstep); inv_head_step.
-  iMod (gen_heap_alloc_gen _ (heap_array l (replicate (Z.to_nat n) v)) with "Hσ")
-    as "(Hσ & Hl & Hm)".
-  { apply heap_array_map_disjoint.
-    rewrite replicate_length Z2Nat.id; auto with lia. }
-  iModIntro; do 2 (iSplit; first done). iFrame "Hσ Hκs". iApply "HΦ".
-  iApply big_sepL_sep. iSplitL "Hl".
-  - by iApply heap_array_to_seq_mapsto.
-  - iApply (heap_array_to_seq_meta with "Hm"). by rewrite replicate_length.
-Qed.
 
 Lemma wp_alloc s E v :
   {{{ True }}} Alloc (Val v) @ s; E {{{ l, RET LitV (LitLoc l); l ↦ v ∗ meta_token l ⊤ }}}.
 Proof.
   iIntros (Φ) "_ HΦ". iApply wp_allocN_seq; auto with lia.
   iIntros "!>" (l) "/= (? & _)". rewrite loc_add_0. iApply "HΦ"; iFrame.
-Qed.
-Lemma twp_alloc s E v :
-  [[{ True }]] Alloc (Val v) @ s; E [[{ l, RET LitV (LitLoc l); l ↦ v ∗ meta_token l ⊤ }]].
-Proof.
-  iIntros (Φ) "_ HΦ". iApply twp_allocN_seq; auto with lia.
-  iIntros (l) "/= (? & _)". rewrite loc_add_0. iApply "HΦ"; iFrame.
 Qed.
 
 Lemma wp_load s E l q v :
@@ -329,14 +278,6 @@ Proof.
   iSplit; first by eauto. iNext; iIntros (v2 σ2 efs Hstep); inv_head_step.
   iModIntro; iSplit=> //. iFrame. by iApply "HΦ".
 Qed.
-Lemma twp_load s E l q v :
-  [[{ l ↦{q} v }]] Load (Val $ LitV $ LitLoc l) @ s; E [[{ RET v; l ↦{q} v }]].
-Proof.
-  iIntros (Φ) "Hl HΦ". iApply twp_lift_atomic_head_step_no_fork; auto.
-  iIntros (σ1 κs n) "[Hσ Hκs] !>". iDestruct (@gen_heap_valid with "Hσ Hl") as %?.
-  iSplit; first by eauto. iIntros (κ v2 σ2 efs Hstep); inv_head_step.
-  iModIntro; iSplit=> //. iSplit; first done. iFrame. by iApply "HΦ".
-Qed.
 
 Lemma wp_store s E l v' v :
   {{{ ▷ l ↦ v' }}} Store (Val $ LitV (LitLoc l)) (Val v) @ s; E
@@ -345,20 +286,10 @@ Proof.
   iIntros (Φ) ">Hl HΦ".
   iApply wp_lift_atomic_head_step_no_fork; auto.
   iIntros (σ1 κ κs n) "[Hσ Hκs] !>". iDestruct (@gen_heap_valid with "Hσ Hl") as %?.
-  iSplit; first by eauto. iNext; iIntros (v2 σ2 efs Hstep); inv_head_step.
+  iSplit; [iPureIntro; left; eauto|].
+  iNext; iIntros (v2 σ2 efs Hstep); inv_head_step.
   iMod (@gen_heap_update with "Hσ Hl") as "[$ Hl]".
   iModIntro. iSplit=>//. iFrame. by iApply "HΦ".
-Qed.
-Lemma twp_store s E l v' v :
-  [[{ l ↦ v' }]] Store (Val $ LitV $ LitLoc l) (Val v) @ s; E
-  [[{ RET LitV LitUnit; l ↦ v }]].
-Proof.
-  iIntros (Φ) "Hl HΦ".
-  iApply twp_lift_atomic_head_step_no_fork; auto.
-  iIntros (σ1 κs n) "[Hσ Hκs] !>". iDestruct (@gen_heap_valid with "Hσ Hl") as %?.
-  iSplit; first by eauto. iIntros (κ v2 σ2 efs Hstep); inv_head_step.
-  iMod (@gen_heap_update with "Hσ Hl") as "[$ Hl]".
-  iModIntro. iSplit=>//. iSplit; first done. iFrame. by iApply "HΦ".
 Qed.
 
 Lemma wp_cmpxchg_fail s E l q v' v1 v2 :
@@ -371,17 +302,6 @@ Proof.
   iSplit; first by eauto. iNext; iIntros (v2' σ2 efs Hstep); inv_head_step.
   rewrite bool_decide_false //.
   iModIntro; iSplit=> //. iFrame. by iApply "HΦ".
-Qed.
-Lemma twp_cmpxchg_fail s E l q v' v1 v2 :
-  v' ≠ v1 → vals_compare_safe v' v1 →
-  [[{ l ↦{q} v' }]] CmpXchg (Val $ LitV $ LitLoc l) (Val v1) (Val v2) @ s; E
-  [[{ RET PairV v' (LitV $ LitBool false); l ↦{q} v' }]].
-Proof.
-  iIntros (?? Φ) "Hl HΦ". iApply twp_lift_atomic_head_step_no_fork; auto.
-  iIntros (σ1 κs n) "[Hσ Hκs] !>". iDestruct (@gen_heap_valid with "Hσ Hl") as %?.
-  iSplit; first by eauto. iIntros (κ v2' σ2 efs Hstep); inv_head_step.
-  rewrite bool_decide_false //.
-  iModIntro; iSplit=> //. iSplit; first done. iFrame. by iApply "HΦ".
 Qed.
 
 Lemma wp_cmpxchg_suc s E l v1 v2 v' :
@@ -396,17 +316,48 @@ Proof.
   iMod (@gen_heap_update with "Hσ Hl") as "[$ Hl]".
   iModIntro. iSplit=>//. iFrame. by iApply "HΦ".
 Qed.
-Lemma twp_cmpxchg_suc s E l v1 v2 v' :
+
+Lemma wp_was_suc s E l v1 v2 v' :
   v' = v1 → vals_compare_safe v' v1 →
-  [[{ l ↦ v' }]] CmpXchg (Val $ LitV $ LitLoc l) (Val v1) (Val v2) @ s; E
-  [[{ RET PairV v' (LitV $ LitBool true); l ↦ v2 }]].
+  {{{ ▷ l ↦ v' }}} WAS (Val $ LitV $ LitLoc l) (Val v1) (Val v2) @ s; E
+  {{{ RET #(); l ↦ v2 }}}.
 Proof.
-  iIntros (?? Φ) "Hl HΦ". iApply twp_lift_atomic_head_step_no_fork; auto.
-  iIntros (σ1 κs n) "[Hσ Hκs] !>". iDestruct (@gen_heap_valid with "Hσ Hl") as %?.
-  iSplit; first by eauto. iIntros (κ v2' σ2 efs Hstep); inv_head_step.
-  rewrite bool_decide_true //.
+  iIntros (?? Φ) ">Hl HΦ". iApply wp_lift_atomic_head_step_no_fork; auto.
+  iIntros (σ1 κ κs n) "[Hσ Hκs] !>". iDestruct (@gen_heap_valid with "Hσ Hl") as %?.
+  iSplit; first by simplify_eq; eauto.
+  iNext. iIntros (v2' σ2 efs  Hstep); inv_head_step.
   iMod (@gen_heap_update with "Hσ Hl") as "[$ Hl]".
-  iModIntro. iSplit=>//. iSplit; first done. iFrame. by iApply "HΦ".
+  iModIntro. iSplit=>//. iFrame. iApply "HΦ". iFrame.
+Qed.
+
+Lemma wp_was_fail s E l q v' v1 v2 :
+  v' ≠ v1 → vals_compare_safe v' v1 →
+  {{{ ▷ l ↦{q} v' }}} WAS (Val $ LitV $ LitLoc l) (Val v1) (Val v2) @ s; E
+  {{{ RET #(); False }}}.
+Proof.
+  iIntros (?? Φ) ">Hl HΦ". iApply wp_lift_atomic_head_step_no_fork; auto.
+  iIntros (σ1 κ κs n) "[Hσ Hκs] !>". iDestruct (@gen_heap_valid with "Hσ Hl") as %?.
+  iSplit.
+  { iPureIntro. right. eapply (Ectx_waiting _ _ [] (WAS #l v1 v2)); first done.
+    eapply WasW; done. }
+  iNext; iIntros (v2' σ2 efs Hstep); inv_head_step.
+Qed.
+
+Lemma wp_was s E l v' v1 v2 :
+  vals_compare_safe v' v1 →
+  {{{ ▷ l ↦ v' }}} WAS (Val $ LitV $ LitLoc l) (Val v1) (Val v2) @ s; E
+  {{{ RET #(); ⌜v' = v1⌝ ∗ l ↦ v2 }}}.
+Proof.
+  iIntros (? Φ) ">Hl HΦ". iApply wp_lift_atomic_head_step_no_fork; auto.
+  iIntros (σ1 κ κs n) "[Hσ Hκs] !>". iDestruct (@gen_heap_valid with "Hσ Hl") as %?.
+  iSplit.
+  { destruct (decide (v' = v1)) eqn:Eqn.
+    - simplify_eq. eauto.
+    - iPureIntro. right. eapply (Ectx_waiting _ _ [] (WAS #l v1 v2)); first done.
+      eapply WasW; done. }
+  iNext. iIntros (v2' σ2 efs  Hstep); inv_head_step.
+  iMod (@gen_heap_update with "Hσ Hl") as "[$ Hl]".
+  iModIntro. iSplit=>//. iFrame. iApply "HΦ". iFrame. done.
 Qed.
 
 Lemma wp_faa s E l i1 i2 :
@@ -418,131 +369,6 @@ Proof.
   iSplit; first by eauto. iNext; iIntros (v2' σ2 efs Hstep); inv_head_step.
   iMod (@gen_heap_update with "Hσ Hl") as "[$ Hl]".
   iModIntro. iSplit=>//. iFrame. by iApply "HΦ".
-Qed.
-Lemma twp_faa s E l i1 i2 :
-  [[{ l ↦ LitV (LitInt i1) }]] FAA (Val $ LitV $ LitLoc l) (Val $ LitV $ LitInt i2) @ s; E
-  [[{ RET LitV (LitInt i1); l ↦ LitV (LitInt (i1 + i2)) }]].
-Proof.
-  iIntros (Φ) "Hl HΦ". iApply twp_lift_atomic_head_step_no_fork; auto.
-  iIntros (σ1 κs n) "[Hσ Hκs] !>". iDestruct (@gen_heap_valid with "Hσ Hl") as %?.
-  iSplit; first by eauto. iIntros (κ e2 σ2 efs Hstep); inv_head_step.
-  iMod (@gen_heap_update with "Hσ Hl") as "[$ Hl]".
-  iModIntro. iSplit=>//. iSplit; first done. iFrame. by iApply "HΦ".
-Qed.
-
-Lemma wp_new_proph s E :
-  {{{ True }}}
-    NewProph @ s; E
-  {{{ pvs p, RET (LitV (LitProphecy p)); proph p pvs }}}.
-Proof.
-  iIntros (Φ) "_ HΦ". iApply wp_lift_atomic_head_step_no_fork; auto.
-  iIntros (σ1 κ κs n) "[Hσ HR] !>". iSplit; first by eauto.
-  iNext; iIntros (v2 σ2 efs Hstep). inv_head_step.
-  iMod (proph_map_new_proph p with "HR") as "[HR Hp]"; first done.
-  iModIntro; iSplit=> //. iFrame. by iApply "HΦ".
-Qed.
-
-(* In the following, strong atomicity is required due to the fact that [e] must
-be able to make a head step for [Resolve e _ _] not to be (head) stuck. *)
-
-Lemma resolve_reducible e σ (p : proph_id) v :
-  Atomic StronglyAtomic e → reducible e σ →
-  reducible (Resolve e (Val (LitV (LitProphecy p))) (Val v)) σ.
-Proof.
-  intros A (κ & e' & σ' & efs & H).
-  exists (κ ++ [(p, (default v (to_val e'), v))]), e', σ', efs.
-  eapply Ectx_step with (K:=[]); try done.
-  assert (∃w, Val w = e') as [w <-].
-  { unfold Atomic in A. apply (A σ e' κ σ' efs) in H. unfold is_Some in H.
-    destruct H as [w H]. exists w. simpl in H. by apply (of_to_val _ _ H). }
-  simpl. constructor. by apply prim_step_to_val_is_head_step.
-Qed.
-
-Lemma step_resolve e vp vt σ1 κ e2 σ2 efs :
-  Atomic StronglyAtomic e →
-  prim_step (Resolve e (Val vp) (Val vt)) σ1 κ e2 σ2 efs →
-  head_step (Resolve e (Val vp) (Val vt)) σ1 κ e2 σ2 efs.
-Proof.
-  intros A [Ks e1' e2' Hfill -> step]. simpl in *.
-  induction Ks as [|K Ks _] using rev_ind.
-  + simpl in *. subst. inversion step. by constructor.
-  + rewrite fill_app /= in Hfill. destruct K; inversion Hfill; subst; clear Hfill.
-    - assert (fill_item K (fill Ks e1') = fill (Ks ++ [K]) e1') as Eq1;
-        first by rewrite fill_app.
-      assert (fill_item K (fill Ks e2') = fill (Ks ++ [K]) e2') as Eq2;
-        first by rewrite fill_app.
-      rewrite fill_app /=. rewrite Eq1 in A.
-      assert (is_Some (to_val (fill (Ks ++ [K]) e2'))) as H.
-      { apply (A σ1 _ κ σ2 efs). eapply Ectx_step with (K0 := Ks ++ [K]); done. }
-      destruct H as [v H]. apply to_val_fill_some in H. by destruct H, Ks.
-    - assert (to_val (fill Ks e1') = Some vp); first by rewrite -H1 //.
-      apply to_val_fill_some in H. destruct H as [-> ->]. inversion step.
-    - assert (to_val (fill Ks e1') = Some vt); first by rewrite -H2 //.
-      apply to_val_fill_some in H. destruct H as [-> ->]. inversion step.
-Qed.
-
-Lemma wp_resolve s E e Φ (p : proph_id) v (pvs : list (val * val)) :
-  Atomic StronglyAtomic e →
-  to_val e = None →
-  proph p pvs -∗
-  WP e @ s; E {{ r, ∀ pvs', ⌜pvs = (r, v)::pvs'⌝ -∗ proph p pvs' -∗ Φ r }} -∗
-  WP Resolve e (Val $ LitV $ LitProphecy p) (Val v) @ s; E {{ Φ }}.
-Proof.
-  (* TODO we should try to use a generic lifting lemma (and avoid [wp_unfold])
-     here, since this breaks the WP abstraction. *)
-  iIntros (A He) "Hp WPe". rewrite !wp_unfold /wp_pre /= He. simpl in *.
-  iIntros (σ1 κ κs n) "[Hσ Hκ]". destruct κ as [|[p' [w' v']] κ' _] using rev_ind.
-  - iMod ("WPe" $! σ1 [] κs n with "[$Hσ $Hκ]") as "[Hs WPe]". iModIntro. iSplit.
-    { iDestruct "Hs" as "%". iPureIntro. destruct s; [ by apply resolve_reducible | done]. }
-    iIntros (e2 σ2 efs step). exfalso. apply step_resolve in step; last done.
-    inversion step. match goal with H: ?κs ++ [_] = [] |- _ => by destruct κs end.
-  - rewrite -app_assoc.
-    iMod ("WPe" $! σ1 _ _ n with "[$Hσ $Hκ]") as "[Hs WPe]". iModIntro. iSplit.
-    { iDestruct "Hs" as %?. iPureIntro. destruct s; [ by apply resolve_reducible | done]. }
-    iIntros (e2 σ2 efs step). apply step_resolve in step; last done.
-    inversion step; simplify_list_eq.
-    iMod ("WPe" $! (Val w') σ2 efs with "[%]") as "WPe".
-    { by eexists [] _ _. }
-    iModIntro. iNext. iMod "WPe" as "[[$ Hκ] WPe]".
-    iMod (proph_map_resolve_proph p' (w',v') κs with "[$Hκ $Hp]") as (vs' ->) "[$ HPost]".
-    iModIntro. rewrite !wp_unfold /wp_pre /=. iDestruct "WPe" as "[HΦ $]".
-    iMod "HΦ". iModIntro. by iApply "HΦ".
-Qed.
-
-(** Lemmas for some particular expression inside the [Resolve]. *)
-Lemma wp_resolve_proph s E (p : proph_id) (pvs : list (val * val)) v :
-  {{{ proph p pvs }}}
-    ResolveProph (Val $ LitV $ LitProphecy p) (Val v) @ s; E
-  {{{ pvs', RET (LitV LitUnit); ⌜pvs = (LitV LitUnit, v)::pvs'⌝ ∗ proph p pvs' }}}.
-Proof.
-  iIntros (Φ) "Hp HΦ". iApply (wp_resolve with "Hp"); first done.
-  iApply wp_pure_step_later=> //=. iApply wp_value.
-  iIntros "!>" (vs') "HEq Hp". iApply "HΦ". iFrame.
-Qed.
-
-Lemma wp_resolve_cmpxchg_suc s E l (p : proph_id) (pvs : list (val * val)) v1 v2 v :
-  vals_compare_safe v1 v1 →
-  {{{ proph p pvs ∗ ▷ l ↦ v1 }}}
-    Resolve (CmpXchg #l v1 v2) #p v @ s; E
-  {{{ RET (v1, #true) ; ∃ pvs', ⌜pvs = ((v1, #true)%V, v)::pvs'⌝ ∗ proph p pvs' ∗ l ↦ v2 }}}.
-Proof.
-  iIntros (Hcmp Φ) "[Hp Hl] HΦ".
-  iApply (wp_resolve with "Hp"); first done.
-  assert (val_is_unboxed v1) as Hv1; first by destruct Hcmp.
-  iApply (wp_cmpxchg_suc with "Hl"); [done..|]. iIntros "!> Hl".
-  iIntros (pvs' ->) "Hp". iApply "HΦ". eauto with iFrame.
-Qed.
-
-Lemma wp_resolve_cmpxchg_fail s E l (p : proph_id) (pvs : list (val * val)) q v' v1 v2 v :
-  v' ≠ v1 → vals_compare_safe v' v1 →
-  {{{ proph p pvs ∗ ▷ l ↦{q} v' }}}
-    Resolve (CmpXchg #l v1 v2) #p v @ s; E
-  {{{ RET (v', #false) ; ∃ pvs', ⌜pvs = ((v', #false)%V, v)::pvs'⌝ ∗ proph p pvs' ∗ l ↦{q} v' }}}.
-Proof.
-  iIntros (NEq Hcmp Φ) "[Hp Hl] HΦ".
-  iApply (wp_resolve with "Hp"); first done.
-  iApply (wp_cmpxchg_fail with "Hl"); [done..|]. iIntros "!> Hl".
-  iIntros (pvs' ->) "Hp". iApply "HΦ". eauto with iFrame.
 Qed.
 
 End lifting.
