theories/heap_lang/tactics.v
@@ -1,4 +1,4 @@
-From iris.heap_lang Require Export lang.
+From diris.heap_lang Require Export lang.
 Set Default Proof Using "Type".
 Import heap_lang.
 
