theories/program_logic/ectx_lifting.v
@@ -11,13 +11,14 @@ Implicit Types Φ : val Λ → iProp Σ.
 Implicit Types v : val Λ.
 Implicit Types e : expr Λ.
 Hint Resolve head_prim_reducible head_reducible_prim_step : core.
+Hint Resolve head_prim_waiting : core.
 Hint Resolve (reducible_not_val _ inhabitant) : core.
 Hint Resolve head_stuck_stuck : core.
 
 Lemma wp_lift_head_step_fupd {s E Φ} e1 :
   to_val e1 = None →
   (∀ σ1 κ κs n, state_interp σ1 (κ ++ κs) n ={E,∅}=∗
-    ⌜head_reducible e1 σ1⌝ ∗
+    ⌜head_reducible e1 σ1 ∨ head_waiting e1 σ1⌝ ∗
     ∀ e2 σ2 efs, ⌜head_step e1 σ1 κ e2 σ2 efs⌝ ={∅,∅,E}▷=∗
       state_interp σ2 κs (length efs + n) ∗
       WP e2 @ s; E {{ Φ }} ∗
@@ -25,15 +26,22 @@ Lemma wp_lift_head_step_fupd {s E Φ} e1 :
   ⊢ WP e1 @ s; E {{ Φ }}.
 Proof.
   iIntros (?) "H". iApply wp_lift_step_fupd=>//. iIntros (σ1 κ κs Qs) "Hσ".
-  iMod ("H" with "Hσ") as "[% H]"; iModIntro.
-  iSplit; first by destruct s; eauto. iIntros (e2 σ2 efs ?).
-  iApply "H"; eauto.
+  iMod ("H" with "Hσ") as (Hrw) "H"; iModIntro.
+  iSplit.
+  - destruct s; last done. iPureIntro. destruct Hrw.
+    + auto.
+    + right. apply head_prim_waiting. done.
+  - iIntros (e2 σ2 efs ?).
+    iApply "H"; eauto.
+    iPureIntro.
+    destruct Hrw; auto.
+    exfalso. eapply head_waiting_prim_step; eauto.
 Qed.
 
 Lemma wp_lift_head_step {s E Φ} e1 :
   to_val e1 = None →
   (∀ σ1 κ κs n, state_interp σ1 (κ ++ κs) n ={E,∅}=∗
-    ⌜head_reducible e1 σ1⌝ ∗
+    ⌜head_reducible e1 σ1 ∨ head_waiting e1 σ1⌝ ∗
     ▷ ∀ e2 σ2 efs, ⌜head_step e1 σ1 κ e2 σ2 efs⌝ ={∅,E}=∗
       state_interp σ2 κs (length efs + n) ∗
       WP e2 @ s; E {{ Φ }} ∗
@@ -68,7 +76,31 @@ Qed.
 Lemma wp_lift_atomic_head_step_fupd {s E1 E2 Φ} e1 :
   to_val e1 = None →
   (∀ σ1 κ κs n, state_interp σ1 (κ ++ κs) n ={E1}=∗
-    ⌜head_reducible e1 σ1⌝ ∗
+    ⌜head_reducible e1 σ1 ∨ head_waiting e1 σ1⌝ ∗
+    ∀ e2 σ2 efs, ⌜head_step e1 σ1 κ e2 σ2 efs⌝ ={E1,E2}▷=∗
+      state_interp σ2 κs (length efs + n) ∗
+      from_option Φ False (to_val e2) ∗
+      [∗ list] ef ∈ efs, WP ef @ s; ⊤ {{ fork_post }})
+  ⊢ WP e1 @ s; E1 {{ Φ }}.
+Proof.
+  iIntros (?) "H". iApply wp_lift_atomic_step_fupd; [done|].
+  iIntros (σ1 κ κs Qs) "Hσ1". iMod ("H" with "Hσ1") as (Hrw) "H". iModIntro.
+  iSplit.
+  - destruct s; last done. iPureIntro. destruct Hrw.
+    + auto.
+    + right. apply head_prim_waiting. done.
+  - iIntros (e2 σ2 efs Hstep).
+    iApply "H"; eauto.
+    iPureIntro.
+    destruct Hrw; auto.
+    exfalso. eapply head_waiting_prim_step; eauto.
+Qed.
+
+(*
+Lemma wp_lift_atomic_head_step_fupd {s E1 E2 Φ} e1 :
+  to_val e1 = None →
+  (∀ σ1 κ κs n, state_interp σ1 (κ ++ κs) n ={E1}=∗
+    ⌜head_reducible e1 σ1 ∨ waiting e1 σ1⌝ ∗
     ∀ e2 σ2 efs, ⌜head_step e1 σ1 κ e2 σ2 efs⌝ ={E1,E2}▷=∗
       state_interp σ2 κs (length efs + n) ∗
       from_option Φ False (to_val e2) ∗
@@ -77,14 +109,15 @@ Lemma wp_lift_atomic_head_step_fupd {s E1 E2 Φ} e1 :
 Proof.
   iIntros (?) "H". iApply wp_lift_atomic_step_fupd; [done|].
   iIntros (σ1 κ κs Qs) "Hσ1". iMod ("H" with "Hσ1") as "[% H]"; iModIntro.
-  iSplit; first by destruct s; auto. iIntros (e2 σ2 efs Hstep).
-  iApply "H"; eauto.
+  iSplit; first by destruct s; naive_solver. iIntros (e2 σ2 efs Hstep).
+  iApply "H"; eauto. destruct H0; auto.
 Qed.
+*)
 
 Lemma wp_lift_atomic_head_step {s E Φ} e1 :
   to_val e1 = None →
   (∀ σ1 κ κs n, state_interp σ1 (κ ++ κs) n ={E}=∗
-    ⌜head_reducible e1 σ1⌝ ∗
+    ⌜head_reducible e1 σ1 ∨ waiting e1 σ1⌝ ∗
     ▷ ∀ e2 σ2 efs, ⌜head_step e1 σ1 κ e2 σ2 efs⌝ ={E}=∗
       state_interp σ2 κs (length efs + n) ∗
       from_option Φ False (to_val e2) ∗
@@ -92,21 +125,27 @@ Lemma wp_lift_atomic_head_step {s E Φ} e1 :
   ⊢ WP e1 @ s; E {{ Φ }}.
 Proof.
   iIntros (?) "H". iApply wp_lift_atomic_step; eauto.
-  iIntros (σ1 κ κs Qs) "Hσ1". iMod ("H" with "Hσ1") as "[% H]"; iModIntro.
-  iSplit; first by destruct s; auto. iNext. iIntros (e2 σ2 efs Hstep).
+  iIntros (σ1 κ κs Qs) "Hσ1". iMod ("H" with "Hσ1") as (Hrw) "H"; iModIntro.
+  iSplit.
+  - destruct s; last done. iPureIntro. destruct Hrw; auto.
+  - iIntros (e2 σ2 efs Hstep).
   iApply "H"; eauto.
+  iPureIntro.
+  destruct Hrw; auto.
+  exfalso. eapply waiting_prim_step; [exact H0 | exact Hstep].
 Qed.
 
 Lemma wp_lift_atomic_head_step_no_fork_fupd {s E1 E2 Φ} e1 :
   to_val e1 = None →
   (∀ σ1 κ κs n, state_interp σ1 (κ ++ κs) n ={E1}=∗
-    ⌜head_reducible e1 σ1⌝ ∗
+    ⌜head_reducible e1 σ1 ∨ head_waiting e1 σ1⌝ ∗
     ∀ e2 σ2 efs, ⌜head_step e1 σ1 κ e2 σ2 efs⌝ ={E1,E2}▷=∗
       ⌜efs = []⌝ ∗ state_interp σ2 κs n ∗ from_option Φ False (to_val e2))
   ⊢ WP e1 @ s; E1 {{ Φ }}.
 Proof.
   iIntros (?) "H". iApply wp_lift_atomic_head_step_fupd; [done|].
-  iIntros (σ1 κ κs Qs) "Hσ1". iMod ("H" $! σ1 with "Hσ1") as "[$ H]"; iModIntro.
+  iIntros (σ1 κ κs Qs) "Hσ1". 
+ iMod ("H" $! σ1 with "Hσ1") as "[$ H]"; iModIntro.
   iIntros (v2 σ2 efs Hstep).
   iMod ("H" $! v2 σ2 efs with "[# //]") as "H".
   iIntros "!> !>". iMod "H" as "(-> & ? & ?) /=". by iFrame.
@@ -115,7 +154,7 @@ Qed.
 Lemma wp_lift_atomic_head_step_no_fork {s E Φ} e1 :
   to_val e1 = None →
   (∀ σ1 κ κs n, state_interp σ1 (κ ++ κs) n ={E}=∗
-    ⌜head_reducible e1 σ1⌝ ∗
+    ⌜head_reducible e1 σ1 ∨ waiting e1 σ1⌝ ∗
     ▷ ∀ e2 σ2 efs, ⌜head_step e1 σ1 κ e2 σ2 efs⌝ ={E}=∗
       ⌜efs = []⌝ ∗ state_interp σ2 κs n ∗ from_option Φ False (to_val e2))
   ⊢ WP e1 @ s; E {{ Φ }}.
